replace riscv.AxiomaticRiscv by compiler.GoFlatToRiscv

compiler/src/GoFlatToRiscv.v
@@ -10,7 +10,7 @@ Require Import riscv.Decode.
 Require Import riscv.Memory.
 Require Import riscv.Program.
 Require Import riscv.RiscvMachine.
-Require Import riscv.AxiomaticRiscv.
+Require Import riscv.Primitives.
 Require Import riscv.Run.
 Require Import riscv.Execute.
 Require Import riscv.proofs.DecodeEncode.
@@ -18,8 +18,9 @@ Require Import coqutil.Tactics.Tactics.
 Require Import compiler.util.Tactics.
 Require Import compiler.SeparationLogic.
 Require Import bedrock2.Scalars.
+Require Import riscv.Encode.
+Require Import riscv.proofs.EncodeBound.
 
-Local Unset Universe Polymorphism.
 
 Section Go.
 
@@ -34,9 +35,121 @@ Section Go.
   Context {M: Type -> Type}.
   Context {MM: Monad M}.
   Context {RVM: RiscvProgram M word}.
-  Context {RVS: @RiscvState M word _ _ RVM}.
-  Context {RVAX: AxiomaticRiscv Action M}.
+  Context {PR: Primitives Action M}.
   Variable iset: InstructionSet.
+
+  Lemma spec_Bind_det{A B: Type}: forall (initialL: RiscvMachineL)
+       (post: B -> RiscvMachineL -> Prop) (m: M A) (f : A -> M B) (a: A) (mid: RiscvMachineL),
+      mcomp_sat m initialL (fun a' mid' => a' = a /\ mid' = mid) ->
+      mcomp_sat (f a) mid post ->
+      mcomp_sat (Bind m f) initialL post.
+  Proof.
+    intros. eapply spec_Bind. eexists. split; [exact H|]. intros. simpl in *.
+    destruct H1. subst. assumption.
+  Qed.
+
+  (* redefine mcomp_sat to simplify for the case where no answer is returned *)
+  Definition mcomp_sat(m: M unit)(initialL: RiscvMachineL)(post: RiscvMachineL -> Prop): Prop :=
+    mcomp_sat m initialL (fun (_: unit) => post).
+
+  Ltac t lem :=
+    intros;
+    try (eapply spec_Bind_det; [|eassumption]); (* try because go_step doesn't need Bind *)
+    apply lem;
+    rewrite_match;
+    eauto.
+
+  Lemma go_getRegister: forall (initialL: RiscvMachineL) (x: Register) v post (f: word -> M unit),
+      valid_register x ->
+      map.get initialL.(getRegs) x = Some v ->
+      mcomp_sat (f v) initialL post ->
+      mcomp_sat (Bind (getRegister x) f) initialL post.
+  Proof. t spec_getRegister. Qed.
+
+  Lemma go_getRegister0: forall (initialL: RiscvMachineL) post (f: word -> M unit),
+      mcomp_sat (f (ZToReg 0)) initialL post ->
+      mcomp_sat (Bind (getRegister Register0) f) initialL post.
+  Proof. t spec_getRegister. Qed.
+
+  Lemma go_setRegister: forall initialL x v post (f: unit -> M unit),
+      valid_register x ->
+      mcomp_sat (f tt) (setRegs initialL (map.put initialL.(getRegs) x v)) post ->
+      mcomp_sat (Bind (setRegister x v) f) initialL post.
+  Proof. t spec_setRegister. Qed.
+
+  Lemma go_setRegister0: forall initialL v post (f: unit -> M unit),
+      mcomp_sat (f tt) initialL post ->
+      mcomp_sat (Bind (setRegister Register0 v) f) initialL post.
+  Proof. t spec_setRegister. Qed.
+
+  Lemma go_loadByte: forall initialL addr (v: w8) (f: w8 -> M unit) post,
+      Memory.loadByte initialL.(getMem) addr = Some v ->
+      mcomp_sat (f v) initialL post ->
+      mcomp_sat (Bind (Program.loadByte addr) f) initialL post.
+  Proof. t spec_loadByte. Qed.
+
+  Lemma go_loadHalf: forall initialL addr (v: w16) (f: w16 -> M unit) post,
+      Memory.loadHalf initialL.(getMem) addr = Some v ->
+      mcomp_sat (f v) initialL post ->
+      mcomp_sat (Bind (Program.loadHalf addr) f) initialL post.
+  Proof. t spec_loadHalf. Qed.
+
+  Lemma go_loadWord: forall initialL addr (v: w32) (f: w32 -> M unit) post,
+      Memory.loadWord initialL.(getMem) addr = Some v ->
+      mcomp_sat (f v) initialL post ->
+      mcomp_sat (Bind (Program.loadWord addr) f) initialL post.
+  Proof. t spec_loadWord. Qed.
+
+  Lemma go_loadDouble: forall initialL addr (v: w64) (f: w64 -> M unit) post,
+      Memory.loadDouble initialL.(getMem) addr = Some v ->
+      mcomp_sat (f v) initialL post ->
+      mcomp_sat (Bind (Program.loadDouble addr) f) initialL post.
+  Proof. t spec_loadDouble. Qed.
+
+  Lemma go_storeByte: forall initialL addr v m' post (f: unit -> M unit),
+        Memory.storeByte initialL.(getMem) addr v = Some m' ->
+        mcomp_sat (f tt) (withMem m' initialL) post ->
+        mcomp_sat (Bind (Program.storeByte addr v) f) initialL post.
+  Proof. t spec_storeByte. Qed.
+
+  Lemma go_storeHalf: forall initialL addr v m' post (f: unit -> M unit),
+        Memory.storeHalf initialL.(getMem) addr v = Some m' ->
+        mcomp_sat (f tt) (withMem m' initialL) post ->
+        mcomp_sat (Bind (Program.storeHalf addr v) f) initialL post.
+  Proof. t spec_storeHalf. Qed.
+
+  Lemma go_storeWord: forall initialL addr v m' post (f: unit -> M unit),
+        Memory.storeWord initialL.(getMem) addr v = Some m' ->
+        mcomp_sat (f tt) (withMem m' initialL) post ->
+        mcomp_sat (Bind (Program.storeWord addr v) f) initialL post.
+  Proof. t spec_storeWord. Qed.
+
+  Lemma go_storeDouble: forall initialL addr v m' post (f: unit -> M unit),
+        Memory.storeDouble initialL.(getMem) addr v = Some m' ->
+        mcomp_sat (f tt) (withMem m' initialL) post ->
+        mcomp_sat (Bind (Program.storeDouble addr v) f) initialL post.
+  Proof. t spec_storeDouble. Qed.
+
+  Lemma go_getPC: forall initialL (f: word -> M unit) post,
+        mcomp_sat (f initialL.(getPc)) initialL post ->
+        mcomp_sat (Bind getPC f) initialL post.
+  Proof. t spec_getPC. Qed.
+
+  Lemma go_setPC: forall initialL v post (f: unit -> M unit),
+        mcomp_sat (f tt) (setNextPc initialL v) post ->
+        mcomp_sat (Bind (setPC v) f) initialL post.
+  Proof. t spec_setPC. Qed.
+
+  Lemma go_step: forall initialL (post: RiscvMachineL -> Prop),
+      post (withNextPc (word.add initialL.(getNextPc) (word.of_Z 4))
+                       (withPc initialL.(getNextPc) initialL)) ->
+      mcomp_sat step initialL post.
+  Proof. t spec_step. Qed.
+
+  Lemma go_done: forall initialL (post: RiscvMachineL -> Prop),
+      post initialL ->
+      mcomp_sat (Return tt) initialL post.
+  Proof. t @spec_Return. Qed.
 
   Lemma go_left_identity{A: Type}: forall initialL post a
          (f : A -> M unit),
@@ -62,9 +175,6 @@ Section Go.
   Proof.
     intros. rewrite associativity. assumption.
   Qed.
-
-  Require Import riscv.Encode.
-  Require Import riscv.proofs.EncodeBound.
 
   Definition ptsto_instr(addr: word)(instr: Instruction): mem -> Prop :=
     scalar Syntax.access_size.four addr (word.of_Z (encode instr)).
